indexing and overall plain type changes in HyE and some changes in dh_hye

examples/crypto/HyE.AE.fst
@@ -19,23 +19,26 @@ open HyE.PlainAE
 let ivsize = aeadRealIVSize AES_128_GCM
 type keysize = aeadKeySize AES_128_GCM
 type aes_key = lbytes keysize (* = b:bytes{B.length b = keysize} *)
-type msg = protected_ae_plain
 type cipher = b:bytes{B.length b >= ivsize}
 (* MK: minimal cipher length twice blocksize? *)
 
-type log_t (i:id) (r:rid) = m_rref r (seq ((msg i) * cipher)) grows
+type log_t (i:ae_id) (r:rid) = m_rref r (seq ((protected_ae_plain i) * cipher)) grows
 
 (**
    The key type is abstract and can only be accessed via the leak and coerce_key functions.
 *)
-noeq abstract type key (i:id) =
-  | Key: #region:rid -> raw:aes_key -> log:log_t i region -> honest:bool-> (key i)
+noeq abstract type key =
+  | Key: #i:ae_id -> #region:rid -> raw:aes_key -> log:log_t i region -> (key)
+
+val get_index: key -> Tot ae_id
+let get_index k =
+  k.i
 
 (** 
     safe_key_gen makes sure that memory safety is preserved while generating a key.
     Also, it makes sure that the log created along with the key is empty.
 *)
-let safe_key_gen #i parent m0 (k:key i) m1 =
+let safe_key_gen parent m0 (k:key) m1 =
     modifies Set.empty m0 m1
   /\ extends k.region parent
   /\ fresh_region k.region m0.h m1.h
@@ -46,7 +49,7 @@ let safe_key_gen #i parent m0 (k:key i) m1 =
    This function generates a key in a fresh region of memory below the parent region.
    The postcondition ensures that the log is empty after creation.
 *)
-val keygen: #i:id -> parent:rid -> ST (key i)
+val keygen: #i:pke_id -> parent:rid -> ST (k:key{fst k.i = i})
   (requires (fun _ -> True))
   (ensures  (fun h0 k h1 -> 
     safe_key_gen parent h0 k h1
@@ -54,14 +57,15 @@ val keygen: #i:id -> parent:rid -> ST (key i)
 let keygen #i parent =
   let raw = random keysize in
   let region = new_region parent in
+  let ae_i = i,fresh_ae_id i in
   let log = alloc_mref_seq region createEmpty in
-  Key #i #region raw log true
+  Key #ae_i #region raw log
 
 (**
    The leak_key function transforms an abstract key into a raw aes_key.
    The refinement type on the key makes sure that no honest keys can be leaked.
 *)
-val leak_key: #i:id -> k:key i{not (honest i)} -> Tot aes_key 
+val leak_key: #i:ae_id -> k:key{not (ae_honest k.i)} -> Tot aes_key 
 let leak_key #i k =
   k.raw
 
@@ -70,13 +74,13 @@ let leak_key #i k =
    as we need to allocate space in memory for the key. The refinement type on the key makes sure that
    abstract keys created this way can not be honest.
 *)
-val coerce_key: i:id{not (honest i) } -> parent:rid -> aes_key -> ST (key i)
+val coerce_key: i:ae_id{not (ae_honest i) } -> parent:rid -> aes_key -> ST (k:key{k.i=i})
   (requires (fun _ -> True))
   (ensures  (safe_key_gen parent))
 let coerce_key i parent raw = 
   let region = new_region parent in
   let log = alloc_mref_seq region createEmpty in
-  Key #i #region raw log false
+  Key #i #region raw log
 
 (**
    safe_log_append makes sure that new entries added to the log are appended in a memory-safe way.
@@ -89,15 +93,15 @@ type safe_log_append k entry h0 h1 =
 (**
    Encrypt a a message under a key. Idealize if the key is honest and ae_ind_cca true.
 *)
-val encrypt: #(i:id) -> (k:key i) -> (m:msg i) -> ST cipher
+val encrypt: #(i:ae_id) -> (k:key{k.i=i} ) -> (m:protected_ae_plain i) -> ST cipher
   (requires (fun h0 -> True
     (*m_contains k.log h0*)))
   (ensures  (fun h0 c h1 -> 
     safe_log_append k (m,c) h0 h1 ))
-let encrypt #i k m : cipher =
+let encrypt #i k m =
   m_recall k.log;
   let iv = random ivsize in
-  let p = if (ae_ind_cca && honest i) then createBytes (length m) 0z else (repr m) in
+  let p = if (ae_ind_cca && ae_honest i) then createBytes (length m) 0z else (repr m) in
   let c = CoreCrypto.aead_encrypt AES_128_GCM k.raw iv empty_bytes p in
   let c = iv@|c in
   write_at_end k.log (m,c);
@@ -108,14 +112,14 @@ let encrypt #i k m : cipher =
    try to obtain the ciphertext from the log. Else decrypt via concrete implementation.
    TODO: Make this a total function.
 *)
-val decrypt: #(i:id) -> (k:key i) -> c:cipher -> ST (option (msg i))
+val decrypt: #(i:ae_id) -> (k:key{k.i=i}) -> c:cipher -> ST (option (protected_ae_plain i))
   (requires (fun h -> True (* Could require Map.contains h0 k.region *)))
   (ensures  (fun h0 res h1 -> //True))
     modifies_none h0 h1
     ///\ ( (b2t ae_ind_cca /\ honest i /\ Some? res) ==> SeqProperties.mem (Some?.v res,c) (m_sel h0 k.log) )
     ))
 let decrypt #i k c =
-  if ae_ind_cca && honest i then
+  if ae_ind_cca && ae_honest i then
     let log = m_read k.log in
     match seq_find (fun mc -> snd mc = c) log with
     | Some mc -> Some (fst mc)
