examples/crypto/HyE.Indexing.fsti
@@ -1,9 +1,16 @@
 module HyE.Indexing
 
-abstract type id = UInt32.t
-abstract type pke_id = UInt32.t
+type pke_id = UInt32.t
+type ae_id = pke_id*UInt32.t
 
-val honest: id -> Tot bool
+
+// Do lookups in the global table here
 val pke_honest: pke_id -> Tot bool
+val ae_honest: i:ae_id -> Tot (b:bool{b ==> pke_honest (fst i)})
 
-assume Index_hasEq: hasEq id
+val fresh_pke_id: unit -> Tot (i:pke_id{pke_honest i})
+
+val fresh_ae_id: pke_id -> Tot UInt32.t
+val dishonest_ae_id: pk_i:pke_id -> Tot (num:UInt32.t{not (ae_honest (pk_i,num))})
+
+assume Index_hasEq: hasEq pke_id
