examples/crypto/HyE.PlainHPKE.fst
@@ -10,24 +10,32 @@ open Platform.Bytes
 
 open HyE.Flags
 open HyE.Indexing
+open HyE.PlainAE
 
-abstract type protected_hpke_plain = 
-  | Prot_hpke_p: #i:id -> b:bytes -> protected_hpke_plain
+type hpke_plain = Bytes.bytes
+
+abstract type protected_hpke_plain (i:pke_id)= 
+  | Prot_hpke_p: b:hpke_plain -> protected_hpke_plain i
 //assume Plain_hasEq: hasEq protected_hpke_plain
-type hpke_plain = bytes
-
-val get_index: protected_hpke_plain -> Tot id
-let get_index p =
-  p.i
 
 (* two pure functions, never called when ideal *)
-val repr: p:protected_hpke_plain{not (honest p.i) || not hpke_ind_cca} -> Tot (hpke_plain)
-let repr p = p.b
+val repr: #i:pke_id -> p:protected_hpke_plain i{not (pke_honest i) || not hpke_ind_cca} -> Tot (hpke_plain)
+let repr #i p = p.b
 
 // Change this if we want to use signcryption with hpke_int-ctxt
-val coerce: #i:id -> p:hpke_plain{not (honest i) || not hpke_ind_cca} -> Tot (protected_hpke_plain)
+val coerce: #i:pke_id -> p:hpke_plain{not (pke_honest i) || not hpke_ind_cca} -> Tot (protected_hpke_plain i)
 let coerce #i p = 
   Prot_hpke_p #i p
 
-val length: protected_hpke_plain -> Tot nat
-let length p = length p.b
+val hpke_message_wrap: #pk_id:pke_id 
+		     -> #k_id:ae_id 
+		     -> p:protected_hpke_plain pk_id{
+			 pke_honest pk_id && 
+			 ae_honest k_id &&
+			 hpke_ind_cca}
+		     -> Tot (protected_ae_plain k_id)
+let hpke_message_wrap #pk_id #k_id p =
+  PlainAE.ae_message_wrap #k_id p.b
+
+val length: #i:pke_id -> protected_hpke_plain i -> Tot nat
+let length #i p = Bytes.length p.b
