examples/crypto/HyE.PlainPKE.fst
@@ -13,19 +13,16 @@ open FStar.HyperHeap
 open FStar.HyperStack
 open FStar.Monotonic.RRef
 
-noeq type protected_pke_plain =
-  | Prot_pke_p : i:id -> k:AE.key i -> protected_pke_plain
+noeq type protected_pke_plain (i:pke_id) =
+  | Prot_pke_plain : k:AE.key{fst (get_index k) = i} -> protected_pke_plain i
 
-type pke_plain = aes_key 
-
-val get_index: protected_pke_plain -> Tot id
-let get_index p =
-  p.i
+type pke_plain (i:pke_id) = aes_key 
 
 (* two pure functions, never called when ideal *)
-val repr: p:protected_pke_plain{not pke_ind_cca || not (honest p.i)} -> Tot pke_plain
-let repr p = HyE.AE.leak_key p.k
+val repr: #i:pke_id -> p:protected_pke_plain i{not pke_ind_cca || not (pke_honest i)} -> Tot (pke_plain i)
+let repr #i p = HyE.AE.leak_key #(AE.get_index p.k) p.k
 
-val coerce: #i:id{not (honest i)} -> parent:rid -> pke_plain -> St (protected_pke_plain)
-let coerce #i parent p_plain = 
-  Prot_pke_p i (HyE.AE.coerce_key i parent p_plain)
+// Not sure how the ids are supposed to work with coerce...
+val coerce: #num:UInt32.t -> #i:pke_id{not (ae_honest (i,num))} -> parent:rid -> pke_plain i -> St (protected_pke_plain i)
+let coerce #num #i parent p_plain = 
+  Prot_pke_plain (HyE.AE.coerce_key (i,num) parent p_plain)
