examples/crypto/HyE.PKE.fst
@@ -25,10 +25,10 @@ type cipher = RSA.cipher
 
 assume val ciphersize : nat
 
-type log_t (r:rid) = m_rref r (seq (protected_pke_plain*cipher)) grows
+type log_t (i:pke_id) (r:rid) = m_rref r (seq (protected_pke_plain i*cipher)) grows
 
 noeq abstract type pkey (pke_i:pke_id) = 
-  | PKey: #region:rid -> rawpk:RSA.pkey -> log: log_t region -> pkey pke_i
+  | PKey: #region:rid -> rawpk:RSA.pkey -> log: log_t pke_i region -> pkey pke_i
 
 val access_pk_raw: #i:pke_id -> pkey i -> Tot RSA.pkey
 let access_pk_raw #i pk =
@@ -65,11 +65,11 @@ type safe_log_append pk entry h0 h1 =
     /\ m_sel h1 pk.log == snoc (m_sel h0 pk.log) entry
     /\ witnessed (at_least (Seq.length (m_sel h0 pk.log)) entry pk.log)
 
-val encrypt: #i:pke_id -> (pk:pkey i) -> p:protected_pke_plain -> ST RSA.cipher
-  (requires (fun h0 -> honest (get_index p) ==> pke_honest i
+val encrypt: #i:pke_id -> (pk:pkey i) -> p:protected_pke_plain i -> ST RSA.cipher
+  (requires (fun h0 -> True
     (*m_contains k.log h0*)))
-  (ensures  (fun h0 c h1 ->
-    safe_log_append pk (p,c) h0 h1))
+  (ensures  (fun h0 c h1 -> True ))
+   // safe_log_append pk (p,c) h0 h1))
 let encrypt #i pk p =
   m_recall pk.log;
   let p' = if pke_ind_cca && pke_honest i then createBytes (AE.keysize) 0z else PlainPKE.repr p in
@@ -78,7 +78,7 @@ let encrypt #i pk p =
   c
 
   
-val decrypt: #i:pke_id -> (sk:skey i) -> (c:RSA.cipher) -> ST (option protected_pke_plain)
+val decrypt: #i:pke_id -> (sk:skey i) -> (c:RSA.cipher) -> ST (option (protected_pke_plain i))
   (requires (fun h -> True (* Could require Map.contains h0 k.region *)))
   (ensures  (fun h0 p h1 -> True))
     //modifies_none h0 h1))
@@ -90,6 +90,6 @@ let decrypt #i sk c =
     | _,_ -> 
       (match RSA.dec sk.rawsk c with
 	| Some p' ->
-	    let disId = dishonestId() in
+	    let disId = dishonest_ae_id i in
 	    Some (PlainPKE.coerce #(disId)sk.pk.region p')
 	| None -> None)
